Metatheory/STLCext/Types.lean
@@ -19,11 +19,33 @@ Simple types now include:
 
 namespace Metatheory.STLCext
 
+-- TODO Document everything related to STLCspec
+class STLCspec where
+  baseTypes : Type _
+  baseTypeValue : baseTypes → Type _
+  [decEqBase : DecidableEq baseTypes]
+  [reprBase : Repr baseTypes]
+  [decEqValues : ∀ t : baseTypes, DecidableEq (baseTypeValue t)]
+  [reprValues : ∀ t : baseTypes, Repr (baseTypeValue t)]
+
+@[reducible]
+def BaseTypes [inst : STLCspec] := inst.baseTypes
+@[reducible]
+def BaseTypeValue [inst : STLCspec] : BaseTypes → Type _ := inst.baseTypeValue
+
+instance [s : STLCspec] : DecidableEq BaseTypes := s.decEqBase
+instance [s : STLCspec] : Repr BaseTypes := s.reprBase
+instance [s : STLCspec] (t: BaseTypes) : DecidableEq (BaseTypeValue t) := s.decEqValues t
+instance [s : STLCspec] (t: BaseTypes) : Repr (BaseTypeValue t) := s.reprValues t
+
 /-! ## Simple Types with Products and Sums -/
+
+section Spec
+variable [spec: STLCspec]
 
 /-- Simple types: base types, function types, products, sums, and unit -/
 inductive Ty where
-  | base : Nat → Ty        -- Base type indexed by natural number
+  | base : BaseTypes → Ty        -- Base type indexed by natural number
   | arr  : Ty → Ty → Ty    -- Function type A → B
   | prod : Ty → Ty → Ty    -- Product type A × B
   | sum  : Ty → Ty → Ty    -- Sum type A + B
@@ -40,17 +62,6 @@ scoped infixl:75 " ⊗ " => Ty.prod
 scoped infixl:65 " ⊕ " => Ty.sum
 
 namespace Ty
-
-/-! ## Common Base Types -/
-
-/-- Base type 0 (often represents Bool) -/
-abbrev TBool : Ty := base 0
-
-/-- Base type 1 (often represents Nat) -/
-abbrev TNat : Ty := base 1
-
-/-- Unit type -/
-abbrev TUnit : Ty := unit
 
 /-! ## Type Properties -/
 
@@ -94,6 +105,32 @@ def churchBool (A : Ty) : Ty := A ⇒ A ⇒ A
 
 /-- Church natural type: (A → A) → A → A -/
 def churchNat (A : Ty) : Ty := (A ⇒ A) ⇒ A ⇒ A
+
+end Ty
+
+end Spec
+
+/-! ## Common Base Types -/
+
+namespace Ty
+section BaseTypeExamples
+
+local instance exampleSpec : STLCspec where
+  baseTypes := Bool
+  baseTypeValue t := if t then Bool else Nat
+  decEqValues t := match t with | true => inferInstanceAs (DecidableEq Bool) | false => inferInstanceAs (DecidableEq Nat)
+  reprValues t := match t with | true => inferInstanceAs (Repr Bool) | false => inferInstanceAs (Repr Nat)
+
+/-- Base type Bool -/
+abbrev TBool : Ty := base true
+
+/-- Base type Nat -/
+abbrev TNat : Ty := base false
+
+/-- Unit type -/
+abbrev TUnit : Ty := Ty.unit
+
+end BaseTypeExamples
 
 end Ty
 
